@prefix to: <https://w3id.org/temporalobjects/> .

@prefix dcmitype: <http://purl.org/dc/dcmitype/> .
@prefix dcterms: <http://purl.org/dc/terms/> .
@prefix owl: <http://www.w3.org/2002/07/owl#> .
@prefix rdf: <http://www.w3.org/1999/02/22-rdf-syntax-ns#> .
@prefix rdfs: <http://www.w3.org/2000/01/rdf-schema#> .
@prefix sdo: <https://schema.org/> .
@prefix skos: <http://www.w3.org/2004/02/skos/core#> .
@prefix time: <http://www.w3.org/2006/time#> .
@prefix xsd: <http://www.w3.org/2001/XMLSchema#> .


<https://w3id.org/temporalobjects>
    a owl:Ontology ;
    skos:prefLabel "Temporal Objects Ontology" ;
    skos:definition """This ontology defines temporal object classes that replicate GeoSPARQL 1.1's spatial object classes that have no equivalent in the Time Ontology in OWL (OWL Time).

It is intended that this ontology be used to separate temporal objects that are hitherto not separated with use of OWL Time's `TemporalEntity` class for both things with temporal extents (equivalent to spatial geometries but temporal) and things without temporal extents directly but with temporal relations (equivalent to spatial features).""" ;
  dcterms:created "2021-09-25"^^xsd:date ;
  dcterms:creator to:nick ;
  dcterms:modified "2021-09-25"^^xsd:date ;
  dcterms:publisher to:isc ;
  dcterms:license <http://purl.org/NET/rdflicense/cc-by4.0> ;
  dcterms:rights "(c) Nicholas Car, 2021" ;
.

to:nick
    a sdo:Person ;
    sdo:name "Nicholas J. Car" ;
    sdo:affiliation "SURROUND Australia Pty Ltd" , "Australian National University", to:isc ;
    sdo:email "nicholas.car@surroundaustralia.com"^^xsd:anyURI ;
    sdo:url "https://orcid.org/0000-0002-8742-7730"^^xsd:anyURI ;
.

to:isc
    a sdo:Organization ;
    sdo:name "International Stratigraphic Commission" ;
    sdo:url "https://stratigraphy.org"^^xsd:anyURI ;
.

to:TemporalObject
    a rdfs:Class, owl:Class ;
    rdfs:isDefinedBy to: ;
    skos:prefLabel "Temporal Object"@en ;
    skos:definition "The class Spatial Object represents everything that can have a temporal representation. It is superclass of Temporal Feature and OWL Time's Temporal Entity."@en ;
.

to:TemporalFeature
    a rdfs:Class, owl:Class ;
    rdfs:isDefinedBy to: ;
    skos:prefLabel "Temporal Feature"@en ;
    rdfs:subClassOf to:TemporalObject ;
    owl:disjointWith time:TemporalEntity ;
    skos:definition "This class represents the top-level temporal feature type. This class is equivalent to GeoSPARQL's Feature class and is the superclass of all things that have a projection in time - a relation to a Temporal Entity."@en ;
.

to:TemporalObjectCollection
    a owl:Class ;
    rdfs:isDefinedBy to: ;
    skos:prefLabel "Temporal Object Collection" ;
    skos:definition "The class Temporal Object Collection represents any collection of individual Temporal Object instances."@en ;
    rdfs:subClassOf dcmitype:Collection ;
    rdfs:subClassOf [
        a owl:Restriction ;
        owl:allValuesFrom to:TemporalObject ;
        owl:onProperty rdfs:member ;
    ] ;
.

to:TemporalFeatureCollection
    a owl:Class ;
    rdfs:isDefinedBy to: ;
    skos:prefLabel "Temporal Entity Collection" ;
    skos:definition "The class Temporal Entity Collection represents any collection of individual Temporal Feature instances."@en ;
    rdfs:subClassOf to:TemporalObjectCollection ;
    rdfs:subClassOf [
        a owl:Restriction ;
        owl:allValuesFrom to:TemporalFeature ;
        owl:onProperty rdfs:member ;
    ] ;
.

to:TemporalEntityCollection
    a owl:Class ;
    rdfs:isDefinedBy to: ;
    skos:prefLabel "Temporal Entity Collection" ;
    skos:definition "The class Temporal Entity Collection represents any collection of individual Temporal Entitie instances."@en ;
    rdfs:subClassOf to:TemporalObjectCollection ;
    rdfs:subClassOf [
        a owl:Restriction ;
        owl:allValuesFrom time:TemporalEntity ;
        owl:onProperty rdfs:member ;
    ] ;
.
